
对a来说

$ f'(1.1) = 1 / (2 * 0.1) * [-3f(1.1) + 4f(1.2) - f(1.3)] = 17.769705 $

$f'(1.2) = 1 / (2 * 0.1) * [f(1.3) - f(1.1)] = 22.193635$

$f'(1.3) = 1/ 0.2 * [f(1.4) - f(1.2)] = 27.10735$

$f'(1.4) = 1/ 0.2 * [f(1.2) - 4f(1.3) + 3f(1.4)] = 32.51085$

对b

$f'(8.1) = 1 / 0.4 * [-3f(8.1) + 4f(8.3) - f(8.5)] = 3.09205$

$f'(8.3) = 1 / 0.4 * [f(8.5) - f(8.1)] = 3.11615$

$f'(8.5) = 1 / 0.4 * [f(8.7) - f(8.3)] = 3.139975$

$f'(8.7) = 1 / 0.4 * [f(8.3) - 4f(8.5) + 3f(8.7)] = 3.163525$
